lib/lib/Data/Ordering.lean
@@ -1,0 +1,40 @@
+import Lib.Tactic
+
+namespace Ordering
+
+def flip : Ordering → Ordering
+| lt => gt
+| eq => eq
+| gt => lt
+
+instance : DecidableEq Ordering
+  | x, y => by
+cases x <;> cases y <;>
+first
+ | apply isTrue; refl
+ | apply isFalse;
+   intro h; cases h
+
+inductive Spec {α} [LT α] (x y : α) : Ordering → Type
+| isLT : x < y → Spec x y lt
+| isEQ : x = y → Spec x y eq
+| isGT : y < x → Spec x y gt
+
+end Ordering
+
+inductive POrdering [LT α] (x y : α) : Type
+| isLT : x < y → POrdering x y
+| isEQ : x = y → POrdering x y
+| isGT : y < x → POrdering x y
+
+namespace POrdering
+open Ordering
+variable [LT α]
+
+@[inline]
+def toOrdering {x y : α} : POrdering x y → Ordering
+| isLT h => lt
+| isEQ h => eq
+| isGT h => gt
+
+end POrdering
